

Procedure to convert 2D formula into 3D complex formula

Kuan Peng 彭宽 titang78@gmail.com

[Formulae ready to use,](#)

[Theory about nD complex number system,](#)

[Download the theory paper](#)

1.	Basics of the 3D complex number algebra	2
a.	Forms of a 3D complex number	2
b.	Conversion from Cartesian form into abdf form	2
c.	Conversion from Cartesian form into trigonometric form	2
d.	Addition and subtraction	2
e.	Multiplication	2
f.	Division z/c	3
g.	3D complex number to the power 2 and 3: z^2 and z^3 in abdf form.....	3
h.	3D complex number to the power n	3
i.	n^{th} Root	3
j.	Conjugate.....	3
k.	Sign of d for iteration	3
l.	Exponential and logarithm	4
m.	Non trigonometric large power computation	4
n.	Forms of a 4D complex number	4
2.	Derivation of the formulae, 9 April 2022	5
a.	Exponential function, 18 April 2022.....	6
b.	Natural logarithm	6
3.	Summary of the procedure	6

Let $z_2=x+yi$ be the 2D complex variable, we can replace it with the 3D complex $z = x+yi+z.j$ in any equation.

1. Basics of the 3D complex number algebra

a. Forms of a 3D complex number

Trigonometric form	$z = r((\cos \theta + \sin \theta i) \cos \varphi + \sin \varphi j)$	(1)
abdf form	$z = r((a + bi)d + fj)$ with $\cos \theta = a, \sin \theta = b, \cos \varphi = d, \sin \varphi = f$	(2)
Cartesian form	$z = x + yi + z_*j = r(ad + bdi + fj)$	(3)

b. Conversion from Cartesian form into abdf form

The transformed z in abdf form is in (6).

$z = x + yi + z_*j$	$r_{xy} = \sqrt{x^2 + y^2}$	$r = \sqrt{x^2 + y^2 + z_*^2}$	(4)
$a = \frac{x}{r_{xy}}, b = \frac{y}{r_{xy}}, d = \frac{r_{xy}}{r}, f = \frac{z_*}{r}$	(5)	$z = r((a + bi)d + fj)$	(6)

c. Conversion from Cartesian form into trigonometric form

1. Compute the moduli r_{xy} and r using (4)
2. Compute the angles in the order φ first, θ second using (7)
3. z in trigonometric form is in (8)

$z = x + yi + z_*j$	$r_{xy} = \sqrt{x^2 + y^2}$	$r = \sqrt{x^2 + y^2 + z_*^2}$	(4)		
$\varphi = \sin^{-1}\left(\frac{Z_*}{r}\right)$	If $y>0$	$\theta = \cos^{-1}\left(\frac{x}{r_{xy}}\right)$	If $y<0$	$\theta = -\cos^{-1}\left(\frac{x}{r_{xy}}\right)$	(7)
$z = r((\cos \theta + \sin \theta \, i) \cos \varphi + \sin \varphi \, j)$					(8)

d. Addition and subtraction

In Cartesian form

$z = x_z + y_z i + z_{*z} j$	$c = x_c + y_c i + z_c j$	(9)
$z \pm c = (x_z + y_z i + z_{*z} j) + (x_c + y_c i + z_c j) = (x_z \pm x_c) + (y_z \pm y_c) i + (z_{*z} \pm z_c) j$		(10)

In trigonometric form

$z = r_z((\cos \theta_z + \sin \theta_z \textcolor{red}{i}) \cos \varphi_z + \sin \varphi_z \textcolor{red}{j})$	$c = r_c((\cos \theta_c + \sin \theta_c \textcolor{red}{i}) \cos \varphi_c + \sin \varphi_c \textcolor{red}{j})$	(11)
$z \pm c = (r_z \cos \theta_z \cos \varphi_z \pm r_c \cos \theta_c \cos \varphi_c) + (r_z \sin \theta_z \cos \varphi_z \pm r_c \sin \theta_c \cos \varphi_c) \textcolor{red}{i} + (r_z \sin \varphi_z \pm r_c \sin \varphi_c) \textcolor{red}{j}$		(12)

e. Multiplication

• In trigonometric form

1. Take z and c given in (11)
2. Add the angles, the angles of the product equal the sum of that of the factors
3. Multiply the moduli, the product is in (13)

$$z \cdot c = r_z r_c ((\cos(\theta_z + \theta_c) + \sin(\theta_z + \theta_c) i) \cos(\varphi_z + \varphi_c) + \sin(\varphi_z + \varphi_c) j) \quad (13)$$

• In Cartesian form

1. Take z and c given in (9)
2. Convert z and c into abdf form using (4), (5)
3. Use formula (14)

$z = x_z + y_z \textcolor{red}{i} + z_{*z} \textcolor{red}{j}$	$c = x_c + y_c \textcolor{red}{i} + z_c \textcolor{red}{j}$	(9)
$z \cdot c = r_z r_c \left(((a_z a_c - b_z b_c) + (b_z a_c + a_z b_c) \textcolor{red}{i}) (d_z d_c - f_z f_c) + (f_z d_c + d_z f_c) \textcolor{red}{j} \right)$		(14)

• Proprieties of multiplication

Multiplication is commutative: $r_c r_z = r_z r_c$ and $\theta_c + \theta_z = \theta_z + \theta_c$, $\varphi_c + \varphi_z = \varphi_z + \varphi_c$

Multiplication is associative: $(r_c r_z) r_+ = r_c (r_z r_+)$ and $(\theta_c + \theta_z) + \theta_+ = \theta_c + (\theta_z + \theta_+)$, $(\varphi_c + \varphi_z) + \varphi_+ = \varphi_c + (\varphi_z + \varphi_+)$

Multiplication is not distributive over addition, (15). If you have $(A+B)C$ in a 2D equation, you have to compute $AC+BC$, but not $D=A+B$ then $D \cdot C$, because multiplication has to be done before addition, see (16).

$$(A + B)C \neq A \cdot C + B \cdot C \quad (15) \quad (A + B)C \Rightarrow A \cdot C + B \cdot C \quad (16)$$

f. Division z/c

- In trigonometric form

1. Take z and c given in (11)
2. Subtract the angles, angles of the product equal the difference of that of the factors
3. Divide the moduli, the quotient is in (17)

$z = r_z((\cos \theta_z + \sin \theta_z i) \cos \varphi_z + \sin \varphi_z j)$	$c = r_c((\cos \theta_c + \sin \theta_c i) \cos \varphi_c + \sin \varphi_c j)$	(11)
$\frac{z}{c} = \frac{r_z}{r_c}((\cos(\theta_z - \theta_c) + \sin(\theta_z - \theta_c) i) \cos(\varphi_z - \varphi_c) + \sin(\varphi_z - \varphi_c) j)$		(17)

- In Cartesian form

1. Compute the numbers a, b, d, f of z using (18), (19) and those of c using (18), (20)
2. Use formula (21)

$a = x + yi + z_*j$	$r_{xy} = \sqrt{x^2 + y^2}$	$r = \sqrt{x^2 + y^2 + z_*^2}$	(18)		
$z = x_z + y_z i + z_{*z} j$	$a_z = \left(\frac{x}{r_{xy}}\right)_z$	$b_z = \left(\frac{y}{r_{xy}}\right)_z$	$d_z = \left(\frac{r_{xy}}{r}\right)_z$	$f_z = \left(\frac{z_*}{r}\right)_z$	(19)
$c = x_c + y_c i + z_{*c} j$	$a_c = \left(\frac{x}{r_{xy}}\right)_c$	$b_c = -\left(\frac{y}{r_{xy}}\right)_c$	$d_c = \left(\frac{r_{xy}}{r}\right)_c$	$f_c = -\left(\frac{z_*}{r}\right)_c$	(20)
$\frac{z}{c} = \frac{r_z}{r_c}((a_z a_c - b_z b_c) + (b_z a_c + a_z b_c) i) (d_z d_c - f_z f_c) + (f_z d_c + d_z f_c) j$					(21)

g. 3D complex number to the power 2 and 3: z² and z³ in abdf form

1. Compute the numbers a, b, d, f of the number z using (18), (19)
2. Use formulae (22), (23), (24), (25)
3. Resulting z² and z³ are in (23), (25)

Power 2	$a_{p2} = 2a^2 - 1$	$b_{p2} = 2ab$	$d_{p2} = 2d^2 - 1$	$f_{p2} = 2df$	(22)	
	$z^2 = (r^2 a_{p2} d_{p2}) + (r^2 b_{p2} d_{p2}) i + (r^2 f_{p2}) j = x_2 + y_2 i + z_{*2} j$					(23)
Power 3	$a_{\cdot} = 4a^3 - 3a$	$b_{\cdot} = 3b - 4b^3$	$d_{\cdot} = 4d^3 - 3d$	$f_{\cdot} = 3f - 4f^3$	(24)	
	$z^3 = (r^3 a_{\cdot} d_{\cdot}) + (r^3 b_{\cdot} d_{\cdot}) i + (r^3 f_{\cdot}) j = x_3 + y_3 i + z_{*3} j$					(25)

h. 3D complex number to the power n

- zⁿ in trigonometric form

$z = r((\cos \theta + \sin \theta i) \cos \varphi + \sin \varphi j)$	$z^n = r^n((\cos n\theta + \sin n\theta i) \cos n\varphi + \sin n\varphi j)$	(26)
--	--	------

- zⁿ in Cartesian form $z = x + yi + z_*j$

1. Convert z into trigonometric form using (4), (7), (8)
2. Use formula (26)

i. nth Root

$\frac{1}{n} = r^{\frac{1}{n}} \left(\cos \frac{\theta}{n} + \sin \frac{\theta}{n} i \right) \cos \frac{\varphi}{n} + \sin \frac{\varphi}{n} j$	(27)
--	------

j. Conjugate

$z = x + yi + z_*j$	$\bar{z} = x - yi - z_*j$	(28)
$z = r((\cos \theta + \sin \theta i) \cos \varphi + \sin \varphi j)$	$\bar{z} = r((\cos \theta + \sin(-\theta) i) \cos \varphi + \sin(-\varphi) j)$	(29)
$z = r((a + bi)d + fj)$	$\bar{z} = r((a - bi)d - fj)$	(30)
	$\bar{z} = \frac{ z ^2}{z}$	(31)

k. Sign of d for iteration

For φ to rotate in the same direction at nth and n+1th step:

$z_n = x_n + y_n i + z_{*n} j = r_n((a_n + b_n i) d_n + f_n j)$	(32)	$z_{n+1} = f(z_n)$	(33)
$z_{n+1} = x_{n+1} + y_{n+1} i + z_{*n+1} j = r_{n+1}((a_{n+1} + b_{n+1} i) d_{n+1} + f_{n+1} j)$	(34)	$sign(d_{n+1}) = sign(d_n)$	(35)

1. Exponential and logarithm

Exponential	$z = x + y\mathbf{i} + z_*\mathbf{j}$	$e^z = e^x(\cos y + \sin y\mathbf{i}) \cos z_* + \sin z_*\mathbf{j}$	(36)	See (80)(81)
Natural logarithm	$z = r((\cos \theta + \sin \theta\mathbf{i}) \cos \varphi + \sin \varphi\mathbf{j})$	$\log z = \log r + \mathbf{i}\theta + \mathbf{j}\varphi$	(37)	See (82)(83)

m. Non trigonometric large power computation

Multiplication and Complex number z^n with modulus r

$z \cdot c = ((a_z a_c - b_z b_c) + (b_z a_c + a_z b_c)\mathbf{i})(d_z d_c - f_z f_c) + (f_z d_c + d_z f_c)\mathbf{j}$	see (66)	(38)	$z^n = r^n((a_n + b_n\mathbf{i})d_n + f_n\mathbf{j})$	(39)
--	----------	------	---	------

Large Power for unit complex number z

$z^4 = (z^2)^2 = ((2a_2^2 - 1) + 2a_2b_2\mathbf{i})(d_2^2 - 1) + 2d_2f_2\mathbf{j}$	$z^5 = z^2z^3$	(40)	See (38), (22), (23), (24), (25)
$z^6 = (z^3)^2 = ((2a_3^2 - 1) + 2a_3b_3\mathbf{i})(d_3^2 - 1) + 2d_3f_3\mathbf{j}$	$z^7 = z^4z^3$	(41)	
$z^8 = (z^4)^2 = ((2a_4^2 - 1) + 2a_4b_4\mathbf{i})(d_4^2 - 1) + 2d_4f_4\mathbf{j}$		(42)	
$z^9 = (z^3)^3 = (a_3(4a_3^2 - 3) + b_3(3 - 4b_3^2)\mathbf{i})d_3(4d_3^2 - 3) + f_3(3 - 4f_3^2)\mathbf{j}$		(43)	

Recurrent formula for unit complex number z using multiplication formula (38)

$z^1 = (a_1 + b_1\mathbf{i})d_1 + f_1\mathbf{j}$	(44)	see (38)
$z^2 = (a_2 + b_2\mathbf{i})d_2 + f_2\mathbf{j} = ((2a_1^2 - 1) + 2a_1b_1\mathbf{i})(d_1^2 - 1) + 2d_1f_1\mathbf{j}$	(45)	
$z^3 = (a_3 + b_3\mathbf{i})d_3 + f_3\mathbf{j} = ((a_2a_1 - b_2b_1) + (b_2a_1 + a_2b_1)\mathbf{i})(d_2d_1 - f_2f_1) + (f_2d_1 + d_2f_1)\mathbf{j}$	(46)	
$z^{n+1} = (a_{n+1} + b_{n+1}\mathbf{i})d_{n+1} + f_{n+1}\mathbf{j} = ((a_na_1 - b_nb_1) + (b_na_1 + a_nb_1)\mathbf{i})(d_nd_1 - f_nf_1) + (f_nd_1 + d_nf_1)\mathbf{j}$	(47)	

n. Forms of a 4D complex number

Trigonometric form	$z = r((\cos \theta + \sin \theta\mathbf{i}) \cos \varphi + \sin \varphi\mathbf{j}) \cos \phi + \sin \phi\mathbf{k}$	(48)
abdf form	$z = r((a + b\mathbf{i})d + f\mathbf{j})g + l\mathbf{j}$ with $\cos \theta = a, \sin \theta = b, \cos \varphi = d, \sin \varphi = f, \cos \phi = g, \sin \phi = l$	(49)
Cartesian form	$z = x_1 + x_2\mathbf{i} + x_3\mathbf{j} + x_4\mathbf{k} = r(adg + bdgi + fgj + lj)$	(50)

2. Derivation of the formulae, 9 April 2022

1. Common form of a 3D complex number is (51):

$$z = r((\cos \theta + \sin \theta i) \cos \varphi + \sin \varphi j) = r((a + bi)d + fj) = r(ad + bdi + fj) \quad (51)$$

The form $z = x + yi + z_*j$ is converted into expression with r, a, b, d, f

$$z = x + yi + z_*j = rad + rbd i + rfj \quad x = rad \quad y = rbd \quad z_* = rf \quad (52)$$

2. Relation between r, a, b, d, f and θ, φ , obtained by comparing the terms in (51)

$$r = \sqrt{x^2 + y^2 + z_*^2} \quad \cos \theta = a \quad \sin \theta = b \quad \cos \varphi = d \quad \sin \varphi = f \quad (53)$$

Computing the number d from $x + yi + z_*j$, see (52), (53)

$$r_{xy} = \sqrt{x^2 + y^2} = \sqrt{(rad)^2 + (rbd)^2} = rd\sqrt{a^2 + b^2} = r \cos \varphi \sqrt{\cos^2 \theta + \sin^2 \theta} = r \cos \varphi \quad \cos \varphi = \frac{r_{xy}}{r} = d \quad (54)$$

Computing a, b, f from $x + yi + z_*j$, see (52), $\sqrt{a^2 + b^2} = 1$

$$\sin \varphi = f = \frac{z_*}{r} \quad \cos \theta = \frac{x}{r_{xy}} = \frac{rad}{\sqrt{(rad)^2 + (rbd)^2}} = \frac{a}{\sqrt{a^2 + b^2}} = a \quad \sin \theta = \frac{y}{r_{xy}} = \frac{b}{\sqrt{a^2 + b^2}} = b \quad (55)$$

Conversion to a, b, d, f

$$z = x + yi + z_*j \quad r_{xy} = \sqrt{x^2 + y^2} \quad r = \sqrt{x^2 + y^2 + z_*^2} \quad (56)$$

$$z = r((\cos \theta + \sin \theta i) \cos \varphi + \sin \varphi j) = r((a + bi)d + fj) \quad x = rad \quad y = rbd \quad z_* = rf \quad (57)$$

$$a = \frac{x}{r_{xy}} \quad b = \frac{y}{r_{xy}} \quad d = \frac{r_{xy}}{r} \quad f = \frac{z_*}{r} \quad \text{see (54), (55)} \quad (58)$$

3. Multiplication of two 3D complex numbers

$$z = r_z((\cos \theta_z + \sin \theta_z i) \cos \varphi_z + \sin \varphi_z j) \quad c = r_c((\cos \theta_c + \sin \theta_c i) \cos \varphi_c + \sin \varphi_c j) \quad (59)$$

Multiplication consists of multiplying the moduli and adding the angles:

$$z \cdot c = r_z r_c ((\cos(\theta_z + \theta_c) + \sin(\theta_z + \theta_c) i) \cos(\varphi_z + \varphi_c) + \sin(\varphi_z + \varphi_c) j) \quad (60)$$

Correspondence sine cosine $\leftrightarrow a, b, d, f$

$$\cos \theta_z = a_z \quad \sin \theta_z = b_z \quad \cos \varphi_z = d_z \quad \sin \varphi_z = f_z \quad \cos \theta_c = a_c \quad \sin \theta_c = b_c \quad \cos \varphi_c = d_c \quad \sin \varphi_c = f_c \quad (61)$$

Trigonometric sum in (60) expressed in terms of a, b, d, f

$$\begin{aligned} \cos(\theta_z + \theta_c) &= \cos \theta_z \cos \theta_c - \sin \theta_z \sin \theta_c \\ \sin(\theta_z + \theta_c) &= \sin \theta_z \cos \theta_c + \cos \theta_z \sin \theta_c \end{aligned} \quad (62) \quad \begin{aligned} \cos(\theta_z + \theta_c) &= a_z a_c - b_z b_c \\ \sin(\theta_z + \theta_c) &= b_z a_c + a_z b_c \end{aligned} \quad (63)$$

$$\begin{aligned} \cos(\varphi_z + \varphi_c) &= \cos \varphi_z \cos \varphi_c - \sin \varphi_z \sin \varphi_c \\ \sin(\varphi_z + \varphi_c) &= \sin \varphi_z \cos \varphi_c + \cos \varphi_z \sin \varphi_c \end{aligned} \quad (64) \quad \begin{aligned} \cos(\varphi_z + \varphi_c) &= d_z d_c - f_z f_c \\ \sin(\varphi_z + \varphi_c) &= f_z d_c + d_z f_c \end{aligned} \quad (65)$$

Expression of multiplication of $z \cdot c$ (60) in terms of a, b, d, f using (63), (65)

$$z \cdot c = r_z r_c ((a_z a_c - b_z b_c) + (b_z a_c + a_z b_c) i) (d_z d_c - f_z f_c) + (f_z d_c + d_z f_c) j \quad (66)$$

4. Division

$$\cos(-\theta_c) = \frac{x}{r_{xy}} = a_c \quad \sin(-\theta_c) = \frac{-y}{r_{xy}} = b_c \quad \cos(-\varphi_c) = \frac{r_{xy}}{r} = d_c \quad \sin(-\varphi_c) = \frac{-z_*}{r} = f_c \quad (67)$$

Division of z/c (60)

$$\frac{z}{c} = \frac{r_z}{r_c} ((a_z a_c - b_z b_c) + (b_z a_c + a_z b_c) i) (d_z d_c - f_z f_c) + (f_z d_c + d_z f_c) j \quad (68)$$

5. Expression of multiplication of $z \cdot c$ (60) in terms of a, b, d, f using (63), (65)

$$z \cdot c = r_z r_c ((a_z a_c - b_z b_c) + (b_z a_c + a_z b_c) i) (d_z d_c - f_z f_c) + (f_z d_c + d_z f_c) j \quad (69)$$

6. Power of a 3D complex number

$$\begin{aligned} z \cdot z \cdots z &= r_z^n ((\cos(\theta_z + \cdots + \theta_z) + \sin \cos(\theta_z + \cdots + \theta_z) i) \cos(\varphi_z + \cdots + \varphi_z) + \sin(\varphi_z + \cdots + \varphi_z) j) \\ z^n &= r_z^n ((\cos n\theta_z + \sin n\theta_z i) \cos n\varphi_z + \sin n\varphi_z j) \end{aligned} \quad (70)$$

Coefficients a, b, d, f for Power 2 and 3: z_{n+1}^2, z_{n+1}^3

Power 2	$a_{p2} = 2a^2 - 1$	$b_{p2} = 2ab$	$d_{p2} = 2d^2 - 1$	$f_{p2} = 2df$	(71)
$z^2 = (r_z^2 a_{p2} d_{p2}) + (r_z^2 b_{p2} d_{p2})i + (r_z^2 f_{p2})j = x_{n+1} + y_{n+1}i + z_{*n+1}j$					(72)
Power 3	$a_{\cdot} = 4a^3 - 3a$	$b_{\cdot} = 3b - 4b^3$	$d_{\cdot} = 4d^3 - 3d$	$f_{\cdot} = 3f - 4f^3$	(73)
$z_n^3 = (r_n^3 a_{\cdot} d_{\cdot}) + (r_n^3 b_{\cdot} d_{\cdot})i + (r_n^3 f_{\cdot})j = x_{n+1} + y_{n+1}i + z_{*n+1}j$					(74)

7. nth Root

$$\frac{1}{z^n} = r_n^{-1} e^{i\frac{\theta}{n}} e^{j\frac{\varphi}{n}} = r_n^{-1} \left(\cos \frac{\theta}{n} + \sin \frac{\theta}{n} i \right) \cos \frac{\varphi}{n} + \sin \frac{\varphi}{n} j \quad (75)$$

8. Addition of 3D complex numbers

$$z + c = (x_z + y_z i + z_{*z} j) + (x_c + y_c i + z_{*c} j) = (x_z + x_c) + (y_z + y_c) i + (z_{*z} + z_{*c}) j \quad (76)$$

9. Order of algebraic operations

$$(A + B)C = D \cdot C \quad D = A + B \quad (77) \quad A \cdot B + C = D + C \quad D = A \cdot B \quad (78) \quad (A + B)C \neq A \cdot C + B \cdot C \quad (79)$$

The addition A+B should be done before multiplication D·C in (77).

The multiplication A·B should be done before addition D+C in (78).

Multiplication is not distributive over addition, see (79).

a. Exponential function, 18 April 2022

$$z = x + y i + z_{*} j \quad e^z = e^{x+y i+z_{*} j} = e^x e^{y i} e^{z_{*} j} = e^x (\cos y + \sin y i) (\cos z_{*} + \sin z_{*} j) \quad (80)$$

$$e^z = e^x (\cos y + \sin y i) \cos z_{*} + \sin z_{*} j \quad (81)$$

b. Natural logarithm

$$z = x + y i + z_{*} j = r (\cos \theta + \sin \theta i) (\cos \varphi + \sin \varphi j) = r e^{i\theta} e^{j\varphi} \quad (82)$$

$$\log z = \log(r e^{i\theta} e^{j\varphi}) = \log r + i\theta + j\varphi \quad (83)$$

3. Summary of the procedure

- 3D complex number z and r, r_{xy} , a, b, d, f and angles

$$z = x + y i + z_{*} j = r_z ((\cos \theta_z + \sin \theta_z i) \cos \varphi_z + \sin \varphi_z j) \quad a = \frac{x}{r_{xy}} = \cos \theta_z \quad b = \frac{y}{r_{xy}} = \sin \theta_z \quad (84)$$

$$r_{xy} = \sqrt{x^2 + y^2} \quad r = \sqrt{x^2 + y^2 + z_{*}^2} \quad d = \frac{r_{xy}}{r} = \cos \varphi_z \quad f = \frac{z_{*}}{r} = \sin \varphi_z \quad (85)$$

- Computation of the angles must respect this order:
 φ first, θ second.
 - Compute φ_z with z_{*} using (86), because $\cos \varphi_z$ is defined as positive.
 - Compute θ_z with x and y using (87) and (88) because $-\pi < \theta_z < \pi$

$$\cos \varphi_z > 0 \quad -\frac{\pi}{2} < \varphi_z < \frac{\pi}{2} \quad \varphi_z = \sin^{-1} \left(\frac{z_{*}}{r} \right) \quad (86)$$

$$\text{If } y > 0, \quad 0 < \theta_z < \pi \quad \theta_z = \cos^{-1} \left(\frac{x}{r_{xy}} \right) \quad (87)$$

$$\text{If } y < 0, \quad -\pi < \theta_z < 0 \quad \theta_z = -\cos^{-1} \left(\frac{x}{r_{xy}} \right) \quad (88)$$

- Multiplication of z·c

Multiplication is done in terms of a, b, d, f in (89), that in terms of moduli and angles is done in (90). The moduli and angles are computed using (86), (87) and (88). One chooses the convenient formula according to the case.

$$\text{With a, b, d, f} \quad z \cdot c = r_z r_c ((a_z a_c - b_z b_c) + (b_z a_c + a_z b_c) i) (d_z d_c - f_z f_c) + (f_z d_c + d_z f_c) j \quad (89)$$

$$\text{With angles} \quad z \cdot c = r_z r_c ((\cos(\theta_z + \theta_c) + \sin(\theta_z + \theta_c) i) \cos(\varphi_z + \varphi_c) + \sin(\varphi_z + \varphi_c) j) \quad (90)$$

Multiplication is commutative: $r_c r_z = r_z r_c$ and $\theta_c + \theta_z = \theta_z + \theta_c$, $\varphi_c + \varphi_z = \varphi_z + \varphi_c$

Multiplication is associative: $(r_c r_z) r_{+} = r_c (r_z r_{+})$ and $(\theta_c + \theta_z) + \theta_{+} = \theta_c + (\theta_z + \theta_{+})$, $(\varphi_c + \varphi_z) + \varphi_{+} = \varphi_c + (\varphi_z + \varphi_{+})$

- Power of a 3D complex number

$z \cdot z \cdots z = r_z^n ((\cos(\theta_z + \cdots + \theta_z) + \sin \cos(\theta_z + \cdots + \theta_z) i) \cos(\varphi_z + \cdots + \varphi_z) + \sin(\varphi_z + \cdots + \varphi_z) j)$ $= r_z^n ((\cos n\theta_z + \sin n\theta_z i) \cos n\varphi_z + \sin n\varphi_z j)$	
$z^n = (r_z^n \cos n\theta_z \cos n\varphi_z) + (r_z^n \sin n\theta_z \cos n\varphi_z) i + (r_z^n \sin n\varphi_z) j = x_n + y_n i + z_{*n} j$	(91)

Coefficients a, b, d, f for Power 2 and 3: for computing z_{n+1}

Power 2	$a_{p2} = 2a^2 - 1$	$b_{p2} = 2ab$	$d_{p2} = 2d^2 - 1$	$f_{p2} = 2df$	(92)
---------	---------------------	----------------	---------------------	----------------	------

$z^2 = (r^2 a_{p2} d_{p2}) + (r^2 b_{p2} d_{p2}) i + (r^2 f_{p2}) j = x_2 + y_2 i + z_{*2} j$	(93)
---	------

Power 3	$a_{\cdot} = 4a^3 - 3a$	$b_{\cdot} = 3b - 4b^3$	$d_{\cdot} = 4d^3 - 3d$	$f_{\cdot} = 3f - 4f^3$	(94)
---------	-------------------------	-------------------------	-------------------------	-------------------------	------

$z^3 = (r^3 a_{\cdot} d_{\cdot}) + (r^3 b_{\cdot} d_{\cdot}) i + (r^3 f_{\cdot}) j = x_3 + y_3 i + z_{*3} j$	(95)
--	------

Example of Mandelbrot sets to the power 2 and 3

Power 2	$z_{n+1} = z^2 + c = x_2 + y_2 i + z_{*2} j + x_c + y_c i + z_{*c} j = x_{n+1} + y_{n+1} i + z_{*n+1} j$	See (93)	(96)
---------	--	----------	------

Power 3	$z_{n+1} = z^3 + c = x_3 + y_3 i + z_{*3} j + x_c + y_c i + z_{*c} j = x_{n+1} + y_{n+1} i + z_{*n+1} j$	See (95)	(97)
---------	--	----------	------

Go back to (84)

- Order of algebraic operations

Addition must be done before being multiplied, that is, **multiplication is not distributive**.

$(A + B)C = D \cdot C$	$D = A + B$	(98)	$A \cdot B + C = D + C$	$D = A \cdot B$	(99)	$(A + B)C \neq A \cdot C + B \cdot C$	(100)
------------------------	-------------	------	-------------------------	-----------------	------	---------------------------------------	-------